Adds the list type and its associated typing rules + Generalises the deep-handler typing rules

theories/logic/interp.v
@@ -56,11 +56,21 @@ Definition sem_ty_int : sem_ty := (λ v, ∃ n : Z, ⌜ v = #n ⌝)%I.
 Definition tyN := nroot .@ "ty".
 Definition sem_ty_ref (τ : sem_ty): sem_ty := 
   (λ v, ∃ l : loc, ⌜ v = #l ⌝ ∗ 
-                   inv (tyN .@ l) (∃ w, l ↦ w ∗ ⌜ copy_ty τ ⌝ ∗ □ (τ w)))%I.
+                   inv (tyN .@ l) (∃ w, l ↦ w ∗ ⌜ copy_ty τ ⌝ ∗ (τ w)))%I.
 
 (* Product type. *)
 Definition sem_ty_prod (τ κ : sem_ty) : sem_ty := 
   (λ v, ∃ v₁ v₂, ⌜v = (v₁, v₂)%V⌝ ∗ τ v₁ ∗ κ v₂)%I.
+
+Fixpoint is_of_list_type (l : val) (τ : sem_ty) (xs : list val) : (iProp Σ) :=
+  match xs with
+    | [] => ⌜ l = NILV ⌝
+    | x :: xxs => ∃ tl, ⌜ l = CONSV x tl ⌝ ∗ τ x ∗ is_of_list_type tl τ xxs
+  end
+.
+
+(* List type. *)
+Definition sem_ty_list (τ : sem_ty) : sem_ty := (λ v, ∃ xs, is_of_list_type v τ xs)%I.
 
 (* Empty Effect Row. *)
 Definition sem_row_bot : sem_row := iEff_bottom.
@@ -105,6 +115,9 @@ Notation "τ '×' κ" := (sem_ty_prod τ%T κ%T)
 Notation "'Ref' τ" := (sem_ty_ref τ%T) 
   (at level 50) : sem_ty_scope.
 
+Notation "'List' τ" := (sem_ty_list τ%T) 
+  (at level 50) : sem_ty_scope.
+
 Notation "⟨⟩" := sem_row_bot : sem_row_scope.
 Notation "τ ⇒ κ" := (sem_row_eff τ%T κ%T) 
   (at level 100, κ at level 200) : sem_row_scope.
@@ -119,18 +132,18 @@ Notation "τ '-{' ρ '}->' κ" := (sem_ty_uarr τ%T ρ%R κ%T)
 Notation "τ → κ" := (sem_ty_uarr τ%T sem_row_bot κ%T)
   (at level 99, κ at level 200) : sem_ty_scope.
 
-(** The Type Context
+(** The Type Environment
 
-The type context is represented as a list.
-Due to the requirement that a type context Γ is ctx_sem_typed,
+The type environment is represented as a list.
+Due to the requirement that a type environment Γ is env_sem_typed,
 we can utilize the seperation logic's disjointness to argue about
-variables occuring twice in the context.
+variables occuring twice in the environment.
 
-Thus if we have a `ctx_sem_typed Γ vs` assumption and
+Thus if we have a `env_sem_typed Γ vs` assumption and
 the same variable occurs twice in Γ we get that:
 
 ∙ They cannot be of the same non-persistent type (e.g. ref nat):
-  So if we have `ctx_typed (l : ref nat; l : ref nat) vs`,  
+  So if we have `env_typed (l : ref nat; l : ref nat) vs`,  
   since the variables l are the same, we would have
   that l, v ∈ vs, and that ⟦ ref nat ⟧ v ∗ ⟦ ref nat ⟧ v
   But that means we would need to provide that l ↦ w ∗ l ↦ w
@@ -141,29 +154,29 @@ the same variable occurs twice in Γ we get that:
 
 ∙ If they don't have the same type:
   Then `vs` would still have only 1 value for the variable `l` so
-  it would be impossible to provide ctx_typed proof.
+  it would be impossible to provide env_typed proof.
 
 *) 
 
-Notation ctx := (list (string * sem_ty)).
+Notation env := (list (string * sem_ty)).
 
-(** The domain of the context. *)
-Notation ctx_dom := (map fst).
+(** The domain of the environment. *)
+Notation env_dom := (map fst).
 
-Fixpoint ctx_sem_typed (Γ : ctx)
+Fixpoint env_sem_typed (Γ : env)
                        (vs : gmap string val) : iProp Σ :=
   match Γ with
     | [] => emp
     | (x,A) :: Γ' => (∃ v, ⌜ vs !! x = Some v ⌝ ∗ A v) ∗ 
-                     ctx_sem_typed Γ' vs
+                     env_sem_typed Γ' vs
   end.
 
-Lemma ctx_sem_typed_empty vs : ⊢ ctx_sem_typed [] vs.
+Lemma env_sem_typed_empty vs : ⊢ env_sem_typed [] vs.
 Proof. done. Qed.
 
-Lemma ctx_sem_typed_insert Γ vs (x : string) v :
-  x ∉ (ctx_dom Γ) →
-  ctx_sem_typed Γ vs ⊢ ctx_sem_typed Γ (binder_insert x v vs).
+Lemma env_sem_typed_insert Γ vs (x : string) v :
+  x ∉ (env_dom Γ) →
+  env_sem_typed Γ vs ⊢ env_sem_typed Γ (binder_insert x v vs).
 Proof.
   iIntros (Helem) "Henv".
   iInduction Γ as [|[y A] Γ'] "IH"; first done. simpl in *.
@@ -173,30 +186,38 @@ Proof.
     { destruct Helem. by apply elem_of_list_here. }
     by rewrite lookup_insert_ne.
   - iApply "IH"; last done. iPureIntro. 
-    destruct (not_elem_of_cons (ctx_dom Γ') x y) as [[ ] _]; done.
+    destruct (not_elem_of_cons (env_dom Γ') x y) as [[ ] _]; done.
 Qed.
 
-Lemma ctx_sem_typed_app Γ₁ Γ₂ vs :
-  ctx_sem_typed (Γ₁ ++ Γ₂) vs ⊢ 
-  ctx_sem_typed Γ₁ vs ∗ ctx_sem_typed Γ₂ vs.
+Lemma env_sem_typed_app Γ₁ Γ₂ vs :
+  env_sem_typed (Γ₁ ++ Γ₂) vs ⊢ 
+  env_sem_typed Γ₁ vs ∗ env_sem_typed Γ₂ vs.
 Proof. 
   iIntros "HΓ₁₂". iInduction Γ₁ as [|[y A] Γ₁'] "IH"; first (by iFrame).
   simpl in *. 
   iDestruct "HΓ₁₂" as "($ & HΓ₁'₂)". by iApply "IH".
 Qed.
 
-Definition copy_ctx Γ :=
-  ∀ vs, Persistent (ctx_sem_typed Γ vs).
+(* Lemma env_sem_not_in_dom Γ x vs : *)
+(*   x ∉ env_dom Γ → *)
+(*   env_sem_typed Γ vs ⊢ ⌜vs !! x = None⌝. *)
+(* Proof. *) 
+(*   iIntros (Hx) "HΓ". *)
+(*   iInduction Γ as [|y ys] "IH"; simpl. *)
+(*   { i *)
+
+Definition copy_env Γ :=
+  ∀ vs, Persistent (env_sem_typed Γ vs).
 
 
 (* Sub-typing and relations *)
 
 Definition ty_le (A B : sem_ty) := ∀ v, A v ⊢ B v.
 Definition row_le (ρ ρ' : sem_row) := ⊢ iEff_le ρ ρ'.
-Definition ctx_le Γ₁ Γ₂ :=
-  ∀ vs, ctx_sem_typed Γ₁ vs ⊢ ctx_sem_typed Γ₂ vs.
+Definition env_le Γ₁ Γ₂ :=
+  ∀ vs, env_sem_typed Γ₁ vs ⊢ env_sem_typed Γ₂ vs.
 
-Notation "Γ₁ '≤C' Γ₂" := (ctx_le Γ₁ Γ₂) (at level 98).
+Notation "Γ₁ '≤E' Γ₂" := (env_le Γ₁ Γ₂) (at level 98).
 Notation "τ '≤T' κ" := (ty_le τ%T κ%T) (at level 98).
 
 Notation "ρ '≤R' ρ'" := (row_le ρ%R ρ'%R) (at level 98).
@@ -291,39 +312,52 @@ Proof.
   by iApply Hκ₁₂.
 Qed.
 
-Lemma ctx_le_refl Γ : Γ ≤C Γ.
+Lemma ty_le_list (τ₁ τ₂ : sem_ty) :
+  τ₁ ≤T τ₂ →
+  List τ₁ ≤T List τ₂.
+Proof.
+  iIntros (Hτ₁₂ v) "(%xs & Hxs)". iExists xs.
+  iInduction xs as [|x xxs] "IH" forall (v); simpl.
+  { by iDestruct "Hxs" as "->". }
+  iDestruct "Hxs" as "(%tl & -> & Hτ₁ & Hxxs)".
+  iExists tl. iSplitR; first done.
+  iSplitL "Hτ₁"; [by iApply Hτ₁₂|]. 
+  by iApply "IH".
+Qed.
+
+Lemma env_le_refl Γ : Γ ≤E Γ.
 Proof. done. Qed.
 
-Lemma ctx_le_trans Γ₁ Γ₂ Γ₃ : 
-  Γ₁ ≤C Γ₂ →
-  Γ₂ ≤C Γ₃ →
-  Γ₁ ≤C Γ₃.
+Lemma env_le_trans Γ₁ Γ₂ Γ₃ : 
+  Γ₁ ≤E Γ₂ →
+  Γ₂ ≤E Γ₃ →
+  Γ₁ ≤E Γ₃.
 Proof.
   iIntros (HΓ₁₂ HΓ₂₃ vs) "HΓ₁ //=".  
   iApply HΓ₂₃. by iApply HΓ₁₂.
 Qed.
 
-Lemma ctx_le_cons Γ₁ Γ₂ τ₁ τ₂ x :
-  Γ₁ ≤C Γ₂ →
+Lemma env_le_cons Γ₁ Γ₂ τ₁ τ₂ x :
+  Γ₁ ≤E Γ₂ →
   τ₁ ≤T τ₂ →
-  (x, τ₁) :: Γ₁ ≤C (x, τ₂) :: Γ₂.
+  (x, τ₁) :: Γ₁ ≤E (x, τ₂) :: Γ₂.
 Proof.
   iIntros (HΓ₁₂ Hτ₁₂ vs) "//= ((%v & Hlookup & Hv) & HΓ₁)".
   iSplitR "HΓ₁"; last (by iApply HΓ₁₂).
   iExists v. iFrame. by iApply Hτ₁₂.
 Qed.
 
-Lemma ctx_le_copy_contraction Γ x τ :
+Lemma env_le_copy_contraction Γ x τ :
   copy_ty τ →
-  (x, τ) :: Γ ≤C (x, τ) :: (x, τ) :: Γ.
+  (x, τ) :: Γ ≤E (x, τ) :: (x, τ) :: Γ.
 Proof.
   iIntros (Hcpyτ vs) "//= [(%w & -> & Hτ) $]". 
   rewrite Hcpyτ. iDestruct "Hτ" as "#Hτ".
   iSplitL; iExists w; by iSplit.
 Qed.
 
-Lemma ctx_le_swap Γ x y τ κ :
-  (x, τ) :: (y, κ) :: Γ ≤C (y, κ) :: (x, τ) :: Γ.
+Lemma env_le_swap Γ x y τ κ :
+  (x, τ) :: (y, κ) :: Γ ≤E (y, κ) :: (x, τ) :: Γ.
 Proof. iIntros (vs) "($ & $ & $) //=". Qed.
 
 (* Copyable types *)
@@ -373,13 +407,25 @@ Proof.
   apply Hcpyκ. 
 Qed.
 
-Lemma copy_ctx_nil : copy_ctx [].
+Lemma copy_ty_list τ : copy_ty τ → copy_ty (List τ).
+Proof.
+  iIntros (Hcpy v). unfold sem_ty_list.
+  apply bi.exist_persistent. intros xs.
+  revert v. induction xs; intros v; simpl. 
+  { apply bi.pure_persistent. }
+  apply bi.exist_persistent. intros tl.
+  apply bi.sep_persistent.
+  { apply bi.pure_persistent. }
+  by apply bi.sep_persistent.
+Qed.
+
+Lemma copy_env_nil : copy_env [].
 Proof. iIntros (vs). apply bi.emp_persistent. Qed.
 
-Lemma copy_ctx_cons Γ x τ : 
-  copy_ctx Γ →
+Lemma copy_env_cons Γ x τ : 
+  copy_env Γ →
   copy_ty τ →
-  copy_ctx ((x, τ) :: Γ).
+  copy_env ((x, τ) :: Γ).
 Proof. 
   iIntros (HcpyΓ Hcpyτ vs). simpl.
   apply bi.sep_persistent; last done.
@@ -392,12 +438,12 @@ Qed.
 
 (* Semantic typing judgment. *)
 Definition sem_typed 
-  (Γ  : ctx)
+  (Γ  : env)
   (e  : expr)
   (ρ  : sem_row)
   (α  : sem_ty) : Prop :=
     ∀ (vs : gmap string val),
-        ctx_sem_typed Γ vs ⊢ EWP (subst_map vs e) <| ρ |> {{ α }}.
+        env_sem_typed Γ vs ⊢ EWP (subst_map vs e) <| ρ |> {{ α }}.
 
 Notation "Γ ⊨ e : ρ : α" := (sem_typed Γ e%E ρ%R α%T)
   (at level 74, e, ρ, α at next level) : bi_scope.
@@ -407,6 +453,12 @@ Notation "⊨ e : ρ : α" := (sem_typed [] e%E ρ%R α%T)
 
 Open Scope bi_scope.
 Open Scope ieff_scope.
+
+  
+(* Helper Tactics *)
+
+Ltac ewp_bottom := iApply ewp_os_prot_mono; 
+                   [by iApply iEff_le_bottom|].
 
 (* Semantic typing rules. *)
 
@@ -433,26 +485,26 @@ Qed.
 (* Subsumption rule *)
 
 Lemma sem_typed_sub Γ Γ' e ρ ρ' τ τ':
-  Γ' ≤C Γ →
-  ρ  ≤R ρ' → 
-  τ  ≤T τ' →
-  Γ ⊨ e: ρ : τ →
-  Γ' ⊨ e: ρ' : τ'.
+  Γ ≤E Γ' →
+  ρ'  ≤R ρ → 
+  τ'  ≤T τ →
+  Γ' ⊨ e : ρ' : τ' →
+  Γ ⊨ e : ρ : τ.
 Proof.
-  iIntros (HΓle Hρle Hτle He vs) "HΓ' //=".
+  iIntros (HΓle Hρle Hτle He vs) "HΓ //=".
   rewrite HΓle.
   iApply ewp_os_prot_mono.
   { iApply Hρle. }
-  iApply (ewp_mono with "[HΓ']").
+  iApply (ewp_mono with "[HΓ]").
   { by iApply He. }
-  iIntros (v) "Hτ". iModIntro.
+  iIntros (v) "Hτ'". iModIntro.
   by iApply Hτle.
 Qed.
 
 (* λ-calculus rules *)
 
 Lemma sem_typed_lfun Γ x e τ ρ κ: 
-  x ∉ (ctx_dom Γ) →
+  x ∉ (env_dom Γ) →
   (x,τ) :: Γ ⊨ e : ρ : κ →
   Γ ⊨ (λ: x, e) : ⟨⟩ : (τ -{ ρ }-∘ κ).
 Proof.
@@ -462,12 +514,12 @@ Proof.
   iApply He. simpl in *. iSplitL "Hw".
   - iExists w. iFrame. iPureIntro.
     by rewrite lookup_insert.
-  - by iApply ctx_sem_typed_insert.
+  - by iApply env_sem_typed_insert.
 Qed.
 
 Lemma sem_typed_ufun Γ x e τ ρ κ: 
-  x ∉ (ctx_dom Γ) →
-  copy_ctx Γ →
+  x ∉ (env_dom Γ) →
+  copy_env Γ →
   (x,τ) :: Γ ⊨ e : ρ : κ →
   Γ ⊨ (λ: x, e) : ⟨⟩ : (τ -{ ρ }-> κ).
 Proof.
@@ -478,7 +530,7 @@ Proof.
   iApply He. simpl in *. iSplitL "Hw".
   - iExists w. iFrame. iPureIntro.
     by rewrite lookup_insert.
-  - by iApply ctx_sem_typed_insert.
+  - by iApply env_sem_typed_insert.
 Qed.
 
 Lemma sem_typed_app Γ₁ Γ₂ e₁ e₂ τ ρ κ: 
@@ -487,7 +539,7 @@ Lemma sem_typed_app Γ₁ Γ₂ e₁ e₂ τ ρ κ:
   Γ₁ ++ Γ₂ ⊨ (e₁ e₂) : ρ : κ.
 Proof.
   iIntros (He₁ He₂ vs) "HΓ₁₂ //=".
-  rewrite ctx_sem_typed_app.
+  rewrite env_sem_typed_app.
   iDestruct "HΓ₁₂" as "[HΓ₁ HΓ₂]".
   iApply (ewp_bind ([AppRCtx (subst_map vs e₁)])); first done.
   iApply (ewp_mono with "[HΓ₂]").
@@ -505,7 +557,7 @@ Lemma sem_typed_pair Γ₁ Γ₂ e₁ e₂ τ ρ κ:
   Γ₁ ++ Γ₂ ⊨ (e₁,e₂) : ρ : (τ × κ).
 Proof.
   iIntros (He₁ He₂ vs) "HΓ₁₂ //=".
-  rewrite ctx_sem_typed_app.
+  rewrite env_sem_typed_app.
   iDestruct "HΓ₁₂" as "[HΓ₁ HΓ₂]".
   iApply (ewp_bind ([PairRCtx (subst_map vs e₁)])); first done.
   iApply (ewp_mono with "[HΓ₂]").
@@ -519,15 +571,15 @@ Proof.
 Qed.
 
 Lemma sem_typed_pair_elim Γ₁ Γ₂ x₁ x₂ e₁ e₂ τ ρ κ ι: 
-  x₁ ∉ (ctx_dom Γ₂) ->
-  x₂ ∉ (ctx_dom Γ₂) ->
+  x₁ ∉ (env_dom Γ₂) ->
+  x₂ ∉ (env_dom Γ₂) ->
   x₁ ≠ x₂ ->
   Γ₁ ⊨ e₁ : ρ : (τ × κ) →
   (x₁, τ) :: (x₂, κ) :: Γ₂ ⊨ e₂ : ρ : ι →
   Γ₁ ++ Γ₂ ⊨ (let: (x₁, x₂) := e₁ in e₂) : ρ : ι.
 Proof.
   iIntros (Helem₁ Helem₂ Hnex₁₂ He₁ He₂ vs) "HΓ₁₂ //=".
-  rewrite ctx_sem_typed_app.
+  rewrite env_sem_typed_app.
   iDestruct "HΓ₁₂" as "[HΓ₁ HΓ₂]".
   ewp_pure_steps.
   set ex1x2 := (λ: x₁ x₂, subst_map (binder_delete x₂ 
@@ -550,7 +602,66 @@ Proof.
   iSplitL "Hκ".
   { iExists v₂. iFrame. iPureIntro. 
     by rewrite lookup_insert. }
-  by repeat (iApply ctx_sem_typed_insert; first done).
+  by repeat (iApply env_sem_typed_insert; first done).
+Qed.
+
+Inductive typed_un_op : un_op → sem_ty → sem_ty → Prop :=  
+  | typed_un_op_neg : typed_un_op NegOp 𝔹 𝔹
+  | typed_un_op_minus : typed_un_op MinusUnOp ℤ ℤ
+.
+
+Lemma sem_typed_un_op Γ e op τ κ ρ: 
+  typed_un_op op τ κ →
+  Γ ⊨ e : ρ : τ →
+  Γ ⊨ UnOp op e : ρ : κ.
+Proof.
+  iIntros (Hop He vs) "HΓ //=".
+  iApply (ewp_bind [UnOpCtx _]); first done.
+  iApply (ewp_mono with "[HΓ]").
+  { by iApply He. }
+  iIntros (v) "Hv !> //=".
+  destruct op; inversion_clear Hop;
+  iDestruct "Hv" as "(%n & ->)";
+  ewp_pure_steps; eauto.
+Qed.
+
+Inductive typed_bin_op : bin_op → sem_ty → sem_ty → sem_ty → Prop :=  
+  | typed_bin_op_plus : typed_bin_op PlusOp ℤ ℤ ℤ
+  | typed_bin_op_minus : typed_bin_op MinusOp ℤ ℤ ℤ
+  | typed_bin_op_mult : typed_bin_op MultOp ℤ ℤ ℤ
+  | typed_bin_op_quot : typed_bin_op QuotOp ℤ ℤ ℤ
+  | typed_bin_op_rem : typed_bin_op RemOp ℤ ℤ ℤ
+  | typed_bin_op_and : typed_bin_op AndOp 𝔹 𝔹 𝔹
+  | typed_bin_op_or : typed_bin_op OrOp 𝔹 𝔹 𝔹
+  | typed_bin_op_xor : typed_bin_op XorOp 𝔹 𝔹 𝔹
+  | typed_bin_op_shiftl : typed_bin_op ShiftLOp ℤ ℤ ℤ
+  | typed_bin_op_shiftr : typed_bin_op ShiftROp ℤ ℤ ℤ
+  | typed_bin_op_le : typed_bin_op LeOp ℤ ℤ 𝔹
+  | typed_bin_op_lt : typed_bin_op LtOp ℤ ℤ 𝔹
+  | typed_bin_op_Eq : typed_bin_op EqOp ℤ ℤ 𝔹
+.
+
+Lemma sem_typed_bin_op Γ₁ Γ₂ e₁ e₂ op τ κ ι ρ: 
+  typed_bin_op op τ κ ι →
+  Γ₁ ⊨ e₁ : ρ : τ →
+  Γ₂ ⊨ e₂ : ρ : κ →
+  Γ₁ ++ Γ₂ ⊨ BinOp op e₁ e₂ : ρ : ι.
+Proof.
+  iIntros (Hop He₁ He₂ vs) "HΓ₁₂ //=".
+  rewrite env_sem_typed_app.
+  iDestruct "HΓ₁₂" as "[HΓ₁ HΓ₂]".
+  iApply (ewp_bind [BinOpRCtx _ _]); first done.
+  iApply (ewp_mono with "[HΓ₂]").
+  { by iApply He₂. }
+  iIntros (v) "Hv !> //=". 
+  iApply (ewp_bind [BinOpLCtx _ _]); first done.
+  iApply (ewp_mono with "[HΓ₁]").
+  { by iApply He₁. }
+  iIntros (w) "Hw !> //=". 
+  destruct op; inversion_clear Hop;
+    iDestruct "Hv" as "(%n1 & ->)";
+    iDestruct "Hw" as "(%n2 & ->)";
+    ewp_pure_steps; eauto.
 Qed.
 
 Lemma sem_typed_if Γ₁ Γ₂ e₁ e₂ e₃ ρ τ: 
@@ -560,7 +671,7 @@ Lemma sem_typed_if Γ₁ Γ₂ e₁ e₂ e₃ ρ τ:
   Γ₁ ++ Γ₂ ⊨ (if: e₁ then e₂ else e₃) : ρ : τ.
 Proof.
   iIntros (He₁ He₂ He₃ vs) "HΓ₁₂ //=".
-  rewrite ctx_sem_typed_app.
+  rewrite env_sem_typed_app.
   iDestruct "HΓ₁₂" as "[HΓ₁ HΓ₂]".
   iApply (ewp_bind [IfCtx (subst_map vs e₂) (subst_map vs e₃)])
     ;first done.
@@ -572,7 +683,75 @@ Proof.
   - by iApply He₃.
 Qed.
 
-(* reference rules *)
+Lemma sem_typed_nil Γ τ: 
+  Γ ⊨ NIL : ⟨⟩ : List τ.
+Proof.
+  iIntros (vs) "HΓ //=". 
+  ewp_pure_steps. by iExists [].
+Qed.
+
+Lemma sem_typed_cons Γ₁ Γ₂ e₁ e₂ ρ τ: 
+  Γ₁ ⊨ e₁ : ρ : τ →
+  Γ₂ ⊨ e₂ : ρ : List τ →
+  Γ₁ ++ Γ₂ ⊨ CONS e₁ e₂ : ρ : List τ.
+Proof.
+  iIntros (He₁ He₂ vs) "HΓ₁₂ //=". 
+  rewrite env_sem_typed_app.
+  iDestruct "HΓ₁₂" as "(HΓ₁ & HΓ₂)".
+  iApply (ewp_bind [InjRCtx; PairRCtx _]); first done.
+  iApply (ewp_mono with "[HΓ₂]").
+  { by iApply He₂. }
+  iIntros (l) "Hl !> //=".
+  iApply (ewp_bind [InjRCtx; PairLCtx _]); first done.
+  iApply (ewp_mono with "[HΓ₁]"); [by iApply He₁|].
+  iIntros (x) "Hx !> //=". ewp_pure_steps.
+  iDestruct "Hl" as "(%xs & Hxs)".
+  iExists (x :: xs). simpl. iExists l. by iFrame.
+Qed.
+
+Lemma sem_typed_list_match Γ₁ Γ₂ x xs e₁ e₂ e₃ ρ τ κ :
+  x ∉ (env_dom Γ₂) ->
+  xs ∉ (env_dom Γ₂) ->
+  x ≠ xs ->
+  Γ₁ ⊨ e₁ : ρ : List τ →
+  Γ₂ ⊨ e₂ : ρ : κ →
+  ((x, τ) :: (xs, (List τ)%T) :: Γ₂) ⊨ e₃ : ρ : κ →
+  Γ₁ ++ Γ₂ ⊨ list-match: e₁ with 
+                  CONS x => xs => e₃ 
+                | NIL => e₂
+              end : ρ : κ.
+Proof.
+  iIntros (Hx Hxs Hneq He₁ He₂ He₃ vs) "HΓ₁₂ //=".
+  rewrite env_sem_typed_app.
+  iDestruct "HΓ₁₂" as "(HΓ₁ & HΓ₂)".
+  iApply (ewp_bind [CaseCtx _ _]); first done.
+  iApply (ewp_mono with "[HΓ₁]"); [by iApply He₁|].
+  iIntros (v₁) "(%l & Hl) !> //=". destruct l.
+  - iDestruct "Hl" as "->". ewp_pure_steps.
+    iApply (He₂ with "[$HΓ₂]").
+  - simpl. iDestruct "Hl" as "(%tl & -> & Hτ & Htl)". 
+    ewp_pure_steps. rewrite lookup_delete. simpl.
+    rewrite decide_False; [|by intros [_ []]].
+    rewrite decide_True; last done. ewp_pure_steps.
+    rewrite decide_True; [|split; congruence].
+    rewrite delete_commute -subst_map_insert delete_commute.
+    rewrite insert_delete_insert. rewrite subst_map_insert.
+    rewrite subst_subst_ne; [|congruence]. rewrite delete_commute.
+    rewrite -subst_map_insert -delete_insert_ne; try congruence.
+    rewrite -subst_map_insert. iApply He₃. simpl.
+    iSplitL "Hτ".
+    { iExists v. iFrame. by rewrite lookup_insert. }
+    iSplitL "Htl".
+    + iExists tl. unfold sem_ty_list. iSplitR.
+      { rewrite lookup_insert_ne; [|congruence].  
+        by rewrite lookup_insert. }
+      by iExists l.
+    + iApply env_sem_typed_insert; first done.
+      by iApply env_sem_typed_insert; first done.
+Qed.
+
+
+(* Reference rules *)
 
 (* The references that we implement here are always copyable, 
    so we have ∀ τ, copy_ty (Ref τ).
@@ -599,9 +778,8 @@ Proof.
   iIntros (v) "Hτ". iModIntro.
   iApply ewp_alloc. iIntros "!> %l Hl".
   iMod (inv_alloc (tyN.@l) _
-       (∃ w, l ↦ w ∗ ⌜copy_ty τ⌝ ∗ □ τ w)%I with "[Hl Hτ]") as "#Hinv".
-  { iExists v. iFrame. iSplit; first done.
-    by iApply bi.intuitionistic. }
+       (∃ w, l ↦ w ∗ ⌜copy_ty τ⌝ ∗ τ w)%I with "[Hl Hτ]") as "#Hinv".
+  { iExists v. by iFrame. }
   iModIntro. iExists l. by auto.
 Qed.
 
@@ -618,7 +796,8 @@ Proof.
   iMod (inv_acc _ (tyN.@l) with "Hinv") as "[(%w & >Hl & >%Hcpy & HA) Hclose]"; 
     first done.
   iModIntro. iApply (ewp_load with "Hl").
-  iNext. iDestruct "HA" as "#HA". 
+  iNext. unfold copy_ty, Persistent in Hcpy.
+  iDestruct (Hcpy w with "HA") as "#HApers".
   iIntros "Hl !>". simpl.
   iMod ("Hclose" with "[Hl]"); last done.
   iExists w. iFrame. by iSplit.
@@ -630,7 +809,7 @@ Lemma sem_typed_store Γ₁ Γ₂ e₁ e₂ ρ τ:
   Γ₁ ++ Γ₂ ⊨ (e₁ <- e₂) : ρ : ().
 Proof.
   iIntros (He₁ He₂ vs) "HΓ₁₂ //=".
-  rewrite !ctx_sem_typed_app.
+  rewrite !env_sem_typed_app.
   iDestruct "HΓ₁₂" as "(HΓ₁ & HΓ₂)". 
   iApply (ewp_bind [StoreRCtx _]); first done. simpl.
   iApply (ewp_mono with "[HΓ₂]").
@@ -646,8 +825,7 @@ Proof.
   iModIntro. iApply (ewp_store with "Hl").
   iIntros "!> Hl !>". 
   iMod ("Hclose" with "[Hl Hτ]"); last done.
-  iExists v. iFrame. iSplit; first done.
-  by iApply bi.intuitionistic.
+  iExists v. by iFrame. 
 Qed.
 
 (* Effect handling rules *)
@@ -674,7 +852,7 @@ Lemma sem_typed_shallow_try Γ₁ Γ₂ e h r ι κ τ τ':
   Γ₁ ++ Γ₂ ⊨ (TryWith e h r) : (ι ⇒ κ) : τ.
 Proof.
   iIntros (ρ He Hh Hr vs) "HΓ₁₂ //=".
-  rewrite !ctx_sem_typed_app.
+  rewrite !env_sem_typed_app.
   iDestruct "HΓ₁₂" as "(HΓ₁ & HΓ₂)". ewp_pure_steps.
   iApply (ewp_try_with with "[HΓ₁] [HΓ₂]").
   { by iApply He. }
@@ -682,91 +860,51 @@ Proof.
   last (iIntros "HFalse"; by rewrite upcl_bottom).
   - iIntros (v) "Hv //=".
     iApply (ewp_bind [AppLCtx v]); first done.
-    iApply ewp_os_prot_mono; [by iApply iEff_le_bottom|]. 
+    ewp_bottom.
     iApply (ewp_mono with "[HΓ₂]"); [by iApply Hr|].
     iIntros (w) "Hw". iModIntro. simpl.
     by iApply "Hw".
   - rewrite upcl_sem_row_eff.
     iIntros "(%a & -> & Ha & Hκb)".
     iApply (ewp_bind [AppLCtx k; AppLCtx a]); first done.
-    iApply ewp_os_prot_mono; [by iApply iEff_le_bottom|]. 
+    ewp_bottom.
     iApply (ewp_mono with "[HΓ₂]").
     { by iApply Hh. }
     iIntros (h') "Hh'". iModIntro. simpl. 
     iApply (ewp_bind [AppLCtx k]); first done. 
     iApply (ewp_mono with "[Hh' Ha]").
-    { iApply ewp_os_prot_mono; [by iApply iEff_le_bottom|].
-      by iApply "Hh'". }
+    { ewp_bottom. by iApply "Hh'". }
     iIntros (ha) "Hha". iModIntro. simpl.
     iApply "Hha". iIntros (w) "Hw".
     by iApply "Hκb".
 Qed.
 
-(* 
-∙ Why does the handler branch of a deep-try handler need to be a value?
-  Because even though it is typed inside an empty context, we might produce
-   a non-persistent resource (a continuation) while evaluating the closed expression.
-  A counter-example where the handler is an expression and it eventually 
-  leads to a continuation being called twice (so an unsafe expression) follows:
-
-   deep-try (do #();; do #()) with
-     effect (
-       shallow-try do #() with 
-         effect (λ: _ k', λ v k, k' #();; k #())
-         return (λ: _, λ v k, #())
-       end
-     )
-     return (λ v, v) 
-   end
-  ⇝
-   deep-try (do #();; do #()) with
-     effect (
-       shallow-try eff #() ∙ with 
-         effect (λ: () k', λ v k, k' #();; k #())
-         return (λ: _, λ v k, #())
-       end
-     )
-     return (λ v, v) 
-   end
-  ⇝ 
-   deep-try (do #();; do #()) with
-     effect (
-         λ v k, (cont l ∙) #() ;; k #()
-     )
-     return id 
-   end / l ↦ #false
-  ⇝ 
-   deep-try (eff #() (∙ ;; do #())) with
-     effect (
-         λ v k, (cont l ∙) #() ;; k #()
-     )
-     return (λ v, v) 
-   end / l ↦ #false
-  ⇝ 
-   (cont l ∙) #() ;; 
-   deep-try (#() ;; do #()) with
-      effect (λ v k, (cont l ∙) #() ;; k #())
-      return (λ v, v) 
-   end / l ↦ #false
- *)
-Lemma sem_typed_deep_try Γ₁ Γ₂ Γ₃ e (h : val) r ρ' ι κ τ τ': 
-  copy_ctx Γ₂ →
+Lemma sem_typed_deep_try Γ₁ Γ₂ Γ₃ e h r ρ' ι κ τ τ': 
   let ρ := (ι ⇒ κ)%R in
   Γ₁ ⊨ e : ρ : τ →
-  Γ₂ ⊨ (of_val h) : ⟨⟩ : (ι ⊸ (κ -{ ρ' }-∘ τ') -{ ρ' }-∘ τ') →
+  Γ₂ ⊨ h : ⟨⟩ : (ι → (κ -{ ρ' }-∘ τ') -{ ρ' }-> τ') →
   Γ₃ ⊨ r : ⟨⟩ : (τ -{ ρ' }-∘ τ') →
   Γ₁ ++ Γ₂ ++ Γ₃ ⊨ (deep-try: e with effect h | return r end) : ρ' : τ'.
 Proof.
-  iIntros (Hcpy ρ He Hh Hr vs) "HΓ₁₂₃ //=".
-  rewrite !ctx_sem_typed_app. rewrite Hcpy.
-  iDestruct "HΓ₁₂₃" as "(HΓ₁ & #HΓ₂ & HΓ₃)". ewp_pure_steps.
-  set rctx := AppRCtx (deep_try_with (λ: <>, subst_map vs e)%E (subst_map vs h))%E.
-  iApply (ewp_bind [rctx]); first done.
-  iApply ewp_os_prot_mono; [by iApply iEff_le_bottom|].
+
+  iIntros (ρ He Hh Hr vs) "HΓ₁₂₃ //=".
+  rewrite !env_sem_typed_app. 
+  iDestruct "HΓ₁₂₃" as "(HΓ₁ & HΓ₂ & HΓ₃)". ewp_pure_steps.
+  set ctx_r := AppRCtx (deep_try_with (λ: <>, subst_map vs e) 
+                                      (subst_map vs h))%E.
+  iApply (ewp_bind [ctx_r]); first done.
+  ewp_bottom.
   iApply (ewp_mono with "[HΓ₃]").
   { by iApply Hr. }
   iIntros (r') "Hr'". iModIntro. simpl.
   ewp_pure_steps.
+  set ctx_h := [
+    AppLCtx r';
+    AppRCtx (deep_try_with (λ: <>, subst_map vs e))%E].
+  iApply (ewp_bind ctx_h); first done.
+  ewp_bottom.
+  iApply (ewp_mono with "[HΓ₂]"); [by iApply Hh|].
+  iIntros (h') "#Hh'". iModIntro. simpl. ewp_pure_steps.
   iApply (ewp_deep_try_with with "[HΓ₁]").
   { by iApply He. }
   iLöb as "IH".
@@ -777,18 +915,11 @@ Proof.
     by iApply "Hr'".
   - rewrite upcl_sem_row_eff.
     iIntros "(%a & -> & Ha & Hκb)".
-    iApply (ewp_bind [AppLCtx k; AppLCtx a]); first done. 
-    iApply ewp_os_prot_mono; [by iApply iEff_le_bottom|]. 
-    simpl. iApply ewp_mono.
-    { by iApply Hh. }
-    iIntros (h') "Hh'". iModIntro. simpl.
-    iApply (ewp_bind [AppLCtx k]); first done. simpl.
-    iApply ewp_os_prot_mono; [by iApply iEff_le_bottom|]. 
-    iApply (ewp_mono with "[Hh' Ha]").
-    { by iApply "Hh'". }
-    iIntros (h'a) "Hh'a". iModIntro. simpl.
-    iApply "Hh'a". iIntros (w) "Hw".
-    iApply ("Hκb" with "Hw"). iNext.
-    rewrite !deep_handler_unfold. 
+    iApply (ewp_bind [AppLCtx k]); first done. 
+    ewp_bottom. simpl. 
+    iApply (ewp_mono with "[Ha]"); [by iApply "Hh'"|].
+    iIntros (ha) "Hha !>". iApply "Hha".
+    iIntros (w) "Hw". iApply ("Hκb" with "Hw"). 
+    iNext. rewrite !deep_handler_unfold. 
     iApply ("IH" with "Hr'").
   Qed.
