theories/lang/hazel.v
@@ -17,12 +17,26 @@ From affine_tes.lang Require Export subst_map.
 Definition pair_elim :=
   (λ: "x", λ: "f", "f" (Fst "x") (Snd "x"))%V.
 
-Notation ELetPair x1 x2 e1 e2 :=
-  (pair_elim e1 (Lam x1 (Lam x2 e2)))%E.
+Notation ELetPair x1 x2 e1 e2 := (pair_elim e1 (Lam x1 (Lam x2 e2)))%E.
 
 Notation "'let:' '(' x1 ',' x2 ')' := e1 'in' e2" := (ELetPair x1%binder x2%binder e1%E e2%E)
   (at level 200, x1, x2 at level 1, e1, e2 at level 200,
    format "'[' 'let:'  '(' x1 ',' x2 ')'  :=  '[' e1 ']'  'in'  '/' e2 ']'") : expr_scope.
+
+(** Notations for lists. *)
+Notation NIL := (InjL #()) (only parsing).
+Notation NILV := (InjLV #()) (only parsing).
+Notation CONS x xs := (InjR (Pair x xs)) (only parsing).
+Notation CONSV x xs := (InjRV (PairV x xs)) (only parsing).
+
+Notation ListMatch e1 e2 x e3 := 
+  (Case e1 (Lam BAnon e2) (Lam (BNamed x) (App (App e3 (Fst (Var x))) (Snd (Var x))))) (only parsing).
+
+Notation "'list-match:' e1 'with' 'CONS' x => xs => e3 | 'NIL' => e2 'end'" :=
+  (ListMatch e1 e2 x%binder (Lam x%binder (Lam xs%binder e3)))
+  (e1, x, xs, e2, e1 at level 200,
+   format "'[hv' 'list-match:'  e1  'with'  '/  ' '[' 'CONS'  x  =>  xs  =>  '/  ' e3 ']'  '/' '[' |  'NIL'  =>  '/  ' e2 ']'  '/' 'end' ']'") : expr_scope.
+
 
 Global Instance load_atomic (l : loc) :
   Atomic StronglyAtomic (Load $ Val $ LitV $ LitLoc l).
@@ -53,4 +67,3 @@ Proof.
    destruct K as [|Ki K]; try destruct Ki; try naive_solver.
    simpl in H1. simplify_eq. by inversion H2.
 Qed.
-
